src/Solver/TD_Interface.thy
@@ -1,5 +1,5 @@
 theory TD_Interface
-  imports TD_CFG_Core "TD.TD_plain"
+  imports TD_CFG_Core "TD.TD_plain" Constraint_System_Sound
 begin
 
 (* Plain TD backend (join only, no widening). *)
@@ -13,49 +13,91 @@ lemma part_solutionD:
 locale td_cfg_plain_solver = td_cfg_core + TD_plain cfg_T
 begin
 
-definition td_sigma :: "(pp, 'a abs_state) map"
+definition td_sigma_at :: "pp \<Rightarrow> (pp, 'a abs_state) map"
 where
-  "td_sigma = TD_plain_Interp_solve cfg_T (cfg_entry g)"
+  "td_sigma_at v0 = TD_plain_Interp_solve cfg_T v0"
 
-definition td_env :: "pp \<Rightarrow> 'a abs_state"
+definition td_env_at :: "pp \<Rightarrow> pp \<Rightarrow> 'a abs_state"
 where
-  "td_env v = lookup_bot td_sigma v"
+  "td_env_at v0 w = lookup_bot (td_sigma_at v0) w"
 
-lemma td_sigma_solve:
-  "TD_plain_Interp_solve cfg_T (cfg_entry g) = td_sigma"
-  unfolding td_sigma_def by simp
+lemma td_sigma_at_solve:
+  "TD_plain_Interp_solve cfg_T v0 = td_sigma_at v0"
+  unfolding td_sigma_at_def by simp
 
-lemma td_plain_part_solution:
-  assumes dom: "TD_plain.solve_dom cfg_T (cfg_entry g)"
-  shows "part_solution cfg_T (cfg_entry g) td_sigma (reach cfg_T td_sigma (cfg_entry g))"
+lemma td_plain_part_solution_at:
+  assumes dom: "TD_plain.solve_dom cfg_T v0"
+  shows "part_solution cfg_T v0 (td_sigma_at v0) (reach cfg_T (td_sigma_at v0) v0)"
 proof (rule TD_plain_Interp.partial_correctness)
-  show "TD_plain.solve_dom cfg_T (cfg_entry g)"
+  show "TD_plain.solve_dom cfg_T v0"
     by (fact dom)
-  show "TD_plain_Interp_solve cfg_T (cfg_entry g) = td_sigma"
-    by (simp add: td_sigma_solve)
+  show "TD_plain_Interp_solve cfg_T v0 = td_sigma_at v0"
+    by (simp add: td_sigma_at_solve)
 qed
 
-lemma td_env_post_fixpoint:
+lemma td_env_at_eq_le:
+  assumes dom: "TD_plain.solve_dom cfg_T v0"
+  assumes w_reach: "w \<in> reach cfg_T (td_sigma_at v0) v0"
+  shows "(eq cfg_T) w (td_sigma_at v0) \<le> mlup (td_sigma_at v0) w"
+  using part_solutionD[OF td_plain_part_solution_at[OF dom] w_reach] by simp
+
+lemma td_env_at_rhs_le:
   assumes fin: "finite (edges g)"
   assumes cfi: "comp_fun_idem join_abs"
   assumes join_sym: "\<And>x y. join_abs x y = join_abs y x"
-  assumes dom: "TD_plain.solve_dom cfg_T (cfg_entry g)"
-  assumes reach: "\<And>v. v \<in> reach cfg_T td_sigma (cfg_entry g)"
-  shows "is_post_fixpoint g tf join_abs bot_abs s0 td_env"
-proof (rule cfg_env_post_fixpoint[where env=td_env and \<sigma>=td_sigma, OF fin cfi join_sym])
-  show "\<And>w. td_env w = lookup_bot td_sigma w"
-    unfolding td_env_def by simp
-next
-  fix v
-  show "(eq cfg_T) v td_sigma \<le> mlup td_sigma v"
-  proof -
-    have v_reach: "v \<in> reach cfg_T td_sigma (cfg_entry g)"
-      using reach by simp
-    have psol: "part_solution cfg_T (cfg_entry g) td_sigma (reach cfg_T td_sigma (cfg_entry g))"
-      using td_plain_part_solution[OF dom] .
-    show ?thesis
-      using part_solutionD[OF psol v_reach] by simp
-  qed
+  assumes dom: "TD_plain.solve_dom cfg_T v0"
+  assumes w_reach: "w \<in> reach cfg_T (td_sigma_at v0) v0"
+  shows "rhs g tf join_abs bot_abs s0 (td_env_at v0) w \<le> td_env_at v0 w"
+proof -
+  have eq_le: "(eq cfg_T) w (td_sigma_at v0) \<le> mlup (td_sigma_at v0) w"
+    using td_env_at_eq_le[OF dom w_reach] .
+  show ?thesis
+    using eq_le_mlup_imp_rhs_le[OF cfg_T_eq fin cfi join_sym eq_le]
+    unfolding td_env_at_def by simp
+qed
+
+lemma td_env_at_entry_le:
+  assumes fin: "finite (edges g)"
+  assumes cfi: "comp_fun_idem join_abs"
+  assumes join_sym: "\<And>x y. join_abs x y = join_abs y x"
+  assumes join_is_sup: "join_abs = (\<squnion>)"
+  assumes bot_is_bot: "bot_abs = bot"
+  assumes dom: "TD_plain.solve_dom cfg_T v0"
+  assumes entry_path: "cfg_path g (cfg_entry g) es v0"
+  shows "s0 \<le> td_env_at v0 (cfg_entry g)"
+proof -
+  have entry_reach: "cfg_entry g \<in> reach cfg_T (td_sigma_at v0) v0"
+    using cfg_path_node_in_reach[OF fin entry_path] .
+  have rhs_le: "rhs g tf join_abs bot_abs s0 (td_env_at v0) (cfg_entry g)
+    \<le> td_env_at v0 (cfg_entry g)"
+    using td_env_at_rhs_le[OF fin cfi join_sym dom entry_reach] .
+  have s0_rhs: "s0 \<le> rhs g tf join_abs bot_abs s0 (td_env_at v0) (cfg_entry g)"
+    using s0_le_rhs_entry[where env="td_env_at v0", OF fin] join_is_sup bot_is_bot
+    by (simp add: join_is_sup bot_is_bot)
+  show ?thesis
+    using order_trans[OF s0_rhs rhs_le] .
+qed
+
+lemma td_env_at_path_step_le:
+  assumes fin: "finite (edges g)"
+  assumes cfi: "comp_fun_idem join_abs"
+  assumes join_sym: "\<And>x y. join_abs x y = join_abs y x"
+  assumes join_is_sup: "join_abs = (\<squnion>)"
+  assumes bot_is_bot: "bot_abs = bot"
+  assumes dom: "TD_plain.solve_dom cfg_T v0"
+  assumes path: "cfg_path g u ((a, w) # es') v0"
+  shows "apply_tf tf a (td_env_at v0 u) \<le> td_env_at v0 w"
+proof -
+  from path obtain ed: "(u, a, w) \<in> edges g" and p2: "cfg_path g w es' v0"
+    by (cases rule: cfg_path.cases) auto
+  have w_reach: "w \<in> reach cfg_T (td_sigma_at v0) v0"
+    using cfg_path_node_in_reach[OF fin p2] .
+  have le_rhs: "apply_tf tf a (td_env_at v0 u)
+    \<le> rhs g tf join_abs bot_abs s0 (td_env_at v0) w"
+    using apply_tf_le_rhs[where env="td_env_at v0", OF fin ed] join_is_sup bot_is_bot
+    by (simp add: join_is_sup bot_is_bot)
+  show ?thesis
+    using order_trans[OF le_rhs td_env_at_rhs_le[OF fin cfi join_sym dom w_reach]] .
 qed
 
 end
@@ -69,48 +111,23 @@ definition td_analyse ::
      => pp => 'a abs_state"
 where
   "td_analyse c tf join_abs bot_abs s0 v =
-     lookup_bot (TD_plain_Interp_solve (make_rhs_tree (to_cfg c) tf join_abs bot_abs s0)
-                   (cfg_entry (to_cfg c))) v"
+     lookup_bot (TD_plain_Interp_solve (make_rhs_tree (to_cfg c) tf join_abs bot_abs s0) v) v"
 
 lemma td_analyse_def_expand:
   "td_analyse c tf join_abs bot_abs s0 v =
-     lookup_bot (TD_plain_Interp_solve (make_rhs_tree (to_cfg c) tf join_abs bot_abs s0)
-                   (cfg_entry (to_cfg c))) v"
+     lookup_bot (TD_plain_Interp_solve (make_rhs_tree (to_cfg c) tf join_abs bot_abs s0) v) v"
   unfolding td_analyse_def by simp
 
-theorem td_analyse_post_fixpoint:
-  fixes c tf join_abs bot_abs s0
-  assumes fin: "finite (edges (to_cfg c))"
-  assumes cfi: "comp_fun_idem (join_abs :: 'a::bounded_semilattice_sup_bot abs_state \<Rightarrow> 'a abs_state \<Rightarrow> 'a abs_state)"
-  assumes join_sym: "\<And>x y. join_abs x y = join_abs y x"
-  assumes solve_dom:
-    "TD_plain.solve_dom (make_rhs_tree (to_cfg c) tf join_abs bot_abs s0) (cfg_entry (to_cfg c))"
-  assumes cfg_in_reach:
-    "\<And>v::pp. v \<in> reach (make_rhs_tree (to_cfg c) tf join_abs bot_abs s0)
-                    (TD_plain_Interp_solve (make_rhs_tree (to_cfg c) tf join_abs bot_abs s0)
-                      (cfg_entry (to_cfg c)))
-                    (cfg_entry (to_cfg c))"
-  shows "is_post_fixpoint (to_cfg c) tf join_abs bot_abs s0
-           (td_analyse c tf join_abs bot_abs s0)"
+lemma td_analyse_eq_env_at:
+  fixes c and tf :: "'a::bounded_semilattice_sup_bot domain_transfer"
+    and join_abs :: "'a abs_state \<Rightarrow> 'a abs_state \<Rightarrow> 'a abs_state"
+    and bot_abs s0 :: "'a abs_state" and v
+  shows "td_analyse c tf join_abs bot_abs s0 v =
+         td_cfg_plain_solver.td_env_at (to_cfg c) tf join_abs bot_abs s0 v v"
 proof -
   interpret plain: td_cfg_plain_solver "to_cfg c" tf join_abs bot_abs s0 .
-  have dom': "TD_plain.solve_dom plain.cfg_T (cfg_entry (to_cfg c))"
-  proof -
-    have "plain.cfg_T = make_rhs_tree (to_cfg c) tf join_abs bot_abs s0"
-      by (simp add: fun_eq_iff plain.cfg_T_eq)
-    then show ?thesis using solve_dom by simp
-  qed
-  have cfg_T: "plain.cfg_T = make_rhs_tree (to_cfg c) tf join_abs bot_abs s0"
-    by (simp add: fun_eq_iff plain.cfg_T_eq)
-  have env_eq: "td_analyse c tf join_abs bot_abs s0 = plain.td_env"
-    unfolding td_analyse_def plain.td_env_def plain.td_sigma_def
-    using cfg_T
-    by (intro ext, simp)  have reach': "\<And>v. v \<in> reach plain.cfg_T plain.td_sigma (cfg_entry (to_cfg c))"
-    using cfg_in_reach
-    by (simp add: plain.td_sigma_def cfg_T fun_eq_iff)
   show ?thesis
-    unfolding env_eq
-    using plain.td_env_post_fixpoint[OF fin cfi join_sym dom' reach'] .
+    unfolding td_analyse_def plain.td_env_at_def plain.td_sigma_at_def plain.cfg_T_def by simp
 qed
 
 end
