src/Pipeline/Pipeline.thy
@@ -101,19 +101,9 @@ lemma sign_pipeline_sound:
   assumes runs: "runs_to c s t"
     and init_ok: "s \<in> sign_domain.gamma_state (ac_init (sign_analysis_config s))"
     and td_solve_dom:
-      "TD_plain.solve_dom
+      "\<And>v. TD_plain.solve_dom
          (make_rhs_tree (to_cfg c) sign_tf (\<squnion>) bot
-            (ac_init (sign_analysis_config s)))
-         (cfg_entry (to_cfg c))"
-    and td_cfg_in_reach:
-      "\<And>v::pp. v \<in> reach
-         (make_rhs_tree (to_cfg c) sign_tf (\<squnion>) bot
-            (ac_init (sign_analysis_config s)))
-         (TD_plain_Interp_solve
-            (make_rhs_tree (to_cfg c) sign_tf (\<squnion>) bot
-              (ac_init (sign_analysis_config s)))
-            (cfg_entry (to_cfg c)))
-         (cfg_entry (to_cfg c))"
+            (ac_init (sign_analysis_config s))) v"
   shows "t \<in> sign_domain.gamma_state
              (run_analysis (sign_analysis_config s) c (cfg_exit (to_cfg c)))"
 proof -
@@ -121,10 +111,14 @@ proof -
     = td_analyse c sign_tf (\<squnion>) bot
                     (ac_init (sign_analysis_config s))"
     unfolding run_analysis_def sign_analysis_config_def sign_tf_def by simp
+  from runs_to_imp_path[OF runs] obtain es where
+    entry_path: "cfg_path (to_cfg c) (cfg_entry (to_cfg c)) es (cfg_exit (to_cfg c))"
+    and _: "t \<in> edges_collect es {s}"
+    by blast
   show ?thesis
     unfolding run_eq
     using runs_toD[OF runs]
-    by (rule sign_analysis_sound[OF init_ok _ td_solve_dom td_cfg_in_reach])
+    by (rule sign_analysis_sound[OF init_ok _ to_cfg_finite entry_path td_solve_dom])
 qed
 
 (* ── Interval Analysis Pipeline ──────────────────────────────── *)
@@ -150,19 +144,9 @@ lemma ivl_init_in_gamma:
 corollary ivl_pipeline_sound:
   assumes runs: "runs_to c s t"
     and td_solve_dom:
-      "TD_plain.solve_dom
+      "\<And>v. TD_plain.solve_dom
          (make_rhs_tree (to_cfg c) ivl_tf (\<squnion>) bot
-            (ac_init (ivl_analysis_config s)))
-         (cfg_entry (to_cfg c))"
-    and td_cfg_in_reach:
-      "\<And>v::pp. v \<in> reach
-         (make_rhs_tree (to_cfg c) ivl_tf (\<squnion>) bot
-            (ac_init (ivl_analysis_config s)))
-         (TD_plain_Interp_solve
-            (make_rhs_tree (to_cfg c) ivl_tf (\<squnion>) bot
-              (ac_init (ivl_analysis_config s)))
-            (cfg_entry (to_cfg c)))
-         (cfg_entry (to_cfg c))"
+            (ac_init (ivl_analysis_config s))) v"
   shows   "t \<in> ivl_domain.gamma_state
                   (run_analysis (ivl_analysis_config s) c
                      (cfg_exit (to_cfg c)))"
@@ -171,14 +155,18 @@ proof -
     = td_analyse c ivl_tf (\<squnion>) bot
                     (ac_init (ivl_analysis_config s))"
     unfolding run_analysis_def ivl_analysis_config_def ivl_tf_def by simp
+  from runs_to_imp_path[OF runs] obtain es where
+    entry_path: "cfg_path (to_cfg c) (cfg_entry (to_cfg c)) es (cfg_exit (to_cfg c))"
+    and _: "t \<in> edges_collect es {s}"
+    by blast
   show ?thesis
     unfolding run_eq
     using runs_toD[OF runs]
     by (rule interval_analysis_sound
-          [OF ivl_init_in_gamma _ td_solve_dom td_cfg_in_reach])
+          [OF ivl_init_in_gamma _ to_cfg_finite entry_path td_solve_dom])
 qed
 
-(* Point-map invariant (post_fixpoint_sound + td_analyse_post_fixpoint). *)
+(* Point-map invariant (td_analyse_collect_sound, Fix B per-pp). *)
 theorem pipeline_invariant_sound:
   fixes cfg :: "'a::bounded_semilattice_sup_bot analysis_config"
   assumes sound:      "sound_domain (ac_gamma cfg)"
@@ -186,53 +174,38 @@ theorem pipeline_invariant_sound:
   assumes bot_eq:     "ac_bot cfg = (\<lambda>_. bot)"
   assumes tf_sound:   "domain_transfer_sound (ac_gamma cfg) (ac_tf cfg)"
   assumes s_in_gamma: "s \<in> sound_domain.gamma_state (ac_gamma cfg) (ac_init cfg)"
+  assumes entry_reachable:
+    "\<And>v. \<exists>es. cfg_path (to_cfg c) (cfg_entry (to_cfg c)) es v"
   assumes td_solve_dom:
-    "TD_plain.solve_dom
-       (make_rhs_tree (to_cfg c) (ac_tf cfg) (ac_join cfg) (ac_bot cfg) (ac_init cfg))
-       (cfg_entry (to_cfg c))"
-  assumes td_cfg_in_reach:
-    "\<And>v::pp. v \<in> reach
-       (make_rhs_tree (to_cfg c) (ac_tf cfg) (ac_join cfg) (ac_bot cfg) (ac_init cfg))
-       (TD_plain_Interp_solve
-          (make_rhs_tree (to_cfg c) (ac_tf cfg) (ac_join cfg) (ac_bot cfg) (ac_init cfg))
-          (cfg_entry (to_cfg c)))
-       (cfg_entry (to_cfg c))"
+    "\<And>v. TD_plain.solve_dom
+       (make_rhs_tree (to_cfg c) (ac_tf cfg) (ac_join cfg) (ac_bot cfg) (ac_init cfg)) v"
   shows   "\<forall>v. cfg_collect (to_cfg c) {s} v \<le>
                     sound_domain.gamma_state (ac_gamma cfg)
                       (run_analysis cfg c v)"
 proof -
   interpret sd: sound_domain "ac_gamma cfg"
-    using sound .  have join_eq': "ac_join cfg = ((\<squnion>) :: 'a abs_state \<Rightarrow> _ \<Rightarrow> _)"
+    using sound .  from tf_sound
+  have ta: "\<forall>x a sigma. \<forall>sa \<in> sd.gamma_state sigma.
+      sa(x := aval a sa) \<in> sd.gamma_state (tf_assign (ac_tf cfg) x a sigma)"
+    and tb: "\<forall>b sigma. \<forall>sa \<in> sd.gamma_state sigma. bval b sa
+      \<longrightarrow> sa \<in> sd.gamma_state (tf_assume (ac_tf cfg) b sigma)"
+    and tn: "\<forall>b sigma. \<forall>sa \<in> sd.gamma_state sigma. \<not> bval b sa
+      \<longrightarrow> sa \<in> sd.gamma_state (tf_assume_not (ac_tf cfg) b sigma)"
+    unfolding domain_transfer_sound_def by auto
+  have je: "ac_join cfg = ((\<squnion>) :: 'a abs_state \<Rightarrow> _ \<Rightarrow> _)"
     unfolding sup_fun_def using join_eq by simp
-  have bot_eq':  "ac_bot cfg = (bot :: 'a abs_state)"
+  have be: "ac_bot cfg = (bot :: 'a abs_state)"
     unfolding bot_fun_def using bot_eq by simp
-  have cfi: "comp_fun_idem (ac_join cfg)"
-    unfolding join_eq' by (rule join_state_comp_fun_idem)
-  have join_sym: "\<And>x y. ac_join cfg x y = ac_join cfg y x"
-    unfolding join_eq using sup_commute by (auto simp: fun_eq_iff)
-  have pfp: "is_post_fixpoint (to_cfg c) (ac_tf cfg) (ac_join cfg) (ac_bot cfg)
-              (ac_init cfg) (run_analysis cfg c)"
-    unfolding run_analysis_def
-    by (rule td_analyse_post_fixpoint[OF to_cfg_finite cfi join_sym
-              td_solve_dom td_cfg_in_reach])
-  have pfp': "is_post_fixpoint (to_cfg c) (ac_tf cfg) (\<squnion>) bot
-              (ac_init cfg) (run_analysis cfg c)"
-    using pfp join_eq' bot_eq' by simp
+  have dom':
+    "\<And>v. TD_plain.solve_dom
+       (make_rhs_tree (to_cfg c) (ac_tf cfg) (\<squnion>) bot (ac_init cfg)) v"
+    using td_solve_dom unfolding je be by simp
   have S_sub: "{s} \<le> sd.gamma_state (ac_init cfg)"
-    using s_in_gamma by blast
-  from tf_sound have ta: "\<forall>x a sigma. \<forall>s \<in> sd.gamma_state sigma.
-              s(x := aval a s) \<in> sd.gamma_state (tf_assign (ac_tf cfg) x a sigma)"
-    unfolding domain_transfer_sound_def by blast
-  from tf_sound have tb: "\<forall>b sigma. \<forall>s \<in> sd.gamma_state sigma.
-              bval b s \<longrightarrow> s \<in> sd.gamma_state (tf_assume (ac_tf cfg) b sigma)"
-    unfolding domain_transfer_sound_def by blast
-  from tf_sound have tn: "\<forall>b sigma. \<forall>s \<in> sd.gamma_state sigma.
-              \<not> bval b s \<longrightarrow> s \<in> sd.gamma_state (tf_assume_not (ac_tf cfg) b sigma)"
-    unfolding domain_transfer_sound_def by blast
+    using s_in_gamma by auto
   show ?thesis
-    by (rule sd.post_fixpoint_sound[OF to_cfg_finite pfp' S_sub ta tb tn])
+    unfolding run_analysis_def je be
+    by (rule sd.td_analyse_collect_sound[OF ta tb tn S_sub to_cfg_finite entry_reachable dom'])
 qed
-
 (* -- Pipeline Soundness (Per-pp, path-based) -----------------------------
 
    Per-program-point soundness, the canonical top-level result.
@@ -251,30 +224,39 @@ theorem pipeline_sound_path:
   assumes sound:      "sound_domain (ac_gamma cfg)"
   assumes join_eq:    "ac_join cfg = (\<lambda>s1 s2. \<lambda>x. s1 x \<squnion> s2 x)"
   assumes bot_eq:     "ac_bot cfg = (\<lambda>_. bot)"
-  assumes tf_sound:   "domain_transfer_sound (ac_gamma cfg) (ac_tf cfg)"
-  assumes s_in_gamma: "s \<in> sound_domain.gamma_state (ac_gamma cfg) (ac_init cfg)"
+  assumes tf_sound:   "domain_transfer_sound (ac_gamma cfg) (ac_tf cfg)"  assumes s_in_gamma: "s \<in> sound_domain.gamma_state (ac_gamma cfg) (ac_init cfg)"
   assumes td_solve_dom:
-    "TD_plain.solve_dom
-       (make_rhs_tree (to_cfg c) (ac_tf cfg) (ac_join cfg) (ac_bot cfg) (ac_init cfg))
-       (cfg_entry (to_cfg c))"
-  assumes td_cfg_in_reach:
-    "\<And>v::pp. v \<in> reach
-       (make_rhs_tree (to_cfg c) (ac_tf cfg) (ac_join cfg) (ac_bot cfg) (ac_init cfg))
-       (TD_plain_Interp_solve
-          (make_rhs_tree (to_cfg c) (ac_tf cfg) (ac_join cfg) (ac_bot cfg) (ac_init cfg))
-          (cfg_entry (to_cfg c)))
-       (cfg_entry (to_cfg c))"
-  assumes path:     "(to_cfg c) \<turnstile> (cfg_entry (to_cfg c)) \<longrightarrow>\<^bsub>es\<^esub> v"
+    "\<And>v. TD_plain.solve_dom
+       (make_rhs_tree (to_cfg c) (ac_tf cfg) (ac_join cfg) (ac_bot cfg) (ac_init cfg)) v"
+  assumes path:     "cfg_path (to_cfg c) (cfg_entry (to_cfg c)) es v"
   assumes t_in:     "t \<in> edges_collect es {s}"
   shows "t \<in> sound_domain.gamma_state (ac_gamma cfg) (run_analysis cfg c v)"
 proof -
-  have inv: "\<forall>v. cfg_collect (to_cfg c) {s} v \<le>
-                  sound_domain.gamma_state (ac_gamma cfg) (run_analysis cfg c v)"
-    by (rule pipeline_invariant_sound[OF sound join_eq bot_eq tf_sound s_in_gamma
-              td_solve_dom td_cfg_in_reach])
+  interpret sd: sound_domain "ac_gamma cfg"
+    using sound .
+  from tf_sound
+  have ta: "\<forall>x a sigma. \<forall>s \<in> sd.gamma_state sigma.
+      s(x := aval a s) \<in> sd.gamma_state (tf_assign (ac_tf cfg) x a sigma)"
+    and tb: "\<forall>b sigma. \<forall>s \<in> sd.gamma_state sigma. bval b s
+      \<longrightarrow> s \<in> sd.gamma_state (tf_assume (ac_tf cfg) b sigma)"
+    and tn: "\<forall>b sigma. \<forall>s \<in> sd.gamma_state sigma. \<not> bval b s
+      \<longrightarrow> s \<in> sd.gamma_state (tf_assume_not (ac_tf cfg) b sigma)"
+    unfolding domain_transfer_sound_def by auto
+  have je: "ac_join cfg = ((\<squnion>) :: 'a abs_state \<Rightarrow> _ \<Rightarrow> _)"
+    unfolding sup_fun_def using join_eq by simp
+  have be: "ac_bot cfg = (bot :: 'a abs_state)"
+    unfolding bot_fun_def using bot_eq by simp  have S_sub: "{s} \<le> sd.gamma_state (ac_init cfg)"
+    using s_in_gamma by auto
+  have dom': "TD_plain.solve_dom
+      (make_rhs_tree (to_cfg c) (ac_tf cfg) (\<squnion>) bot (ac_init cfg)) v"
+    using td_solve_dom unfolding je be by simp
+  have collect: "cfg_collect (to_cfg c) {s} v
+    \<le> sd.gamma_state (run_analysis cfg c v)"
+    unfolding run_analysis_def je be
+    by (rule sd.td_analyse_collect_sound_at[OF ta tb tn S_sub to_cfg_finite path dom'])
   have t_in_cfg: "t \<in> cfg_collect (to_cfg c) {s} v"
     using path_sound_cfg_collect[OF path] t_in by blast
-  from inv[rule_format, of v] t_in_cfg show ?thesis by blast
+  show ?thesis using collect t_in_cfg by blast
 qed
 
 
@@ -293,24 +275,43 @@ theorem pipeline_sound_runs_to:
   assumes tf_sound:   "domain_transfer_sound (ac_gamma cfg) (ac_tf cfg)"
   assumes s_in_gamma: "s \<in> sound_domain.gamma_state (ac_gamma cfg) (ac_init cfg)"
   assumes td_solve_dom:
-    "TD_plain.solve_dom
-       (make_rhs_tree (to_cfg c) (ac_tf cfg) (ac_join cfg) (ac_bot cfg) (ac_init cfg))
-       (cfg_entry (to_cfg c))"
-  assumes td_cfg_in_reach:
-    "\<And>v::pp. v \<in> reach
-       (make_rhs_tree (to_cfg c) (ac_tf cfg) (ac_join cfg) (ac_bot cfg) (ac_init cfg))
-       (TD_plain_Interp_solve
-          (make_rhs_tree (to_cfg c) (ac_tf cfg) (ac_join cfg) (ac_bot cfg) (ac_init cfg))
-          (cfg_entry (to_cfg c)))
-       (cfg_entry (to_cfg c))"
+    "\<And>v. TD_plain.solve_dom
+       (make_rhs_tree (to_cfg c) (ac_tf cfg) (ac_join cfg) (ac_bot cfg) (ac_init cfg)) v"
   assumes exit_in_collect:
     "t \<in> cfg_collect (to_cfg c) {s} (cfg_exit (to_cfg c))"
   shows "t \<in> sound_domain.gamma_state (ac_gamma cfg)
                   (run_analysis cfg c (cfg_exit (to_cfg c)))"
-  using exit_in_collect pipeline_invariant_sound[OF sound join_eq bot_eq tf_sound
-          s_in_gamma td_solve_dom td_cfg_in_reach, rule_format,
-          of "cfg_exit (to_cfg c)"]
-  by blast
+proof -
+  interpret sd: sound_domain "ac_gamma cfg"
+    using sound .
+  from tf_sound
+  have ta: "\<forall>x a sigma. \<forall>s \<in> sd.gamma_state sigma.
+      s(x := aval a s) \<in> sd.gamma_state (tf_assign (ac_tf cfg) x a sigma)"
+    and tb: "\<forall>b sigma. \<forall>s \<in> sd.gamma_state sigma. bval b s
+      \<longrightarrow> s \<in> sd.gamma_state (tf_assume (ac_tf cfg) b sigma)"
+    and tn: "\<forall>b sigma. \<forall>s \<in> sd.gamma_state sigma. \<not> bval b s
+      \<longrightarrow> s \<in> sd.gamma_state (tf_assume_not (ac_tf cfg) b sigma)"
+    unfolding domain_transfer_sound_def by auto
+  have je: "ac_join cfg = ((\<squnion>) :: 'a abs_state \<Rightarrow> _ \<Rightarrow> _)"
+    unfolding sup_fun_def using join_eq by simp
+  have be: "ac_bot cfg = (bot :: 'a abs_state)"
+    unfolding bot_fun_def using bot_eq by simp
+  have S_sub: "{s} \<le> sd.gamma_state (ac_init cfg)"
+    using s_in_gamma by auto
+  from exit_in_collect
+  have path_mem: "t \<in> cfg_collect_paths (to_cfg c) {s} (cfg_exit (to_cfg c))"
+    by (simp add: cfg_collect_eq_cfg_collect_paths[symmetric])
+  obtain es where entry_path: "cfg_path (to_cfg c) (cfg_entry (to_cfg c)) es (cfg_exit (to_cfg c))"
+    and _: "t \<in> edges_collect es {s}"    using path_mem unfolding cfg_collect_paths_def by auto
+  have dom': "TD_plain.solve_dom
+      (make_rhs_tree (to_cfg c) (ac_tf cfg) (\<squnion>) bot (ac_init cfg)) (cfg_exit (to_cfg c))"
+    using td_solve_dom unfolding je be by simp
+  have collect: "cfg_collect (to_cfg c) {s} (cfg_exit (to_cfg c))
+    \<le> sd.gamma_state (run_analysis cfg c (cfg_exit (to_cfg c)))"
+    unfolding run_analysis_def je be
+    by (rule sd.td_analyse_collect_sound_at[OF ta tb tn S_sub to_cfg_finite entry_path dom'])
+  show ?thesis using collect exit_in_collect by blast
+qed
 
 corollary pipeline_sound_runs_to_runs:
   fixes cfg :: "'a::bounded_semilattice_sup_bot analysis_config"
@@ -320,43 +321,25 @@ corollary pipeline_sound_runs_to_runs:
   assumes tf_sound:   "domain_transfer_sound (ac_gamma cfg) (ac_tf cfg)"
   assumes s_in_gamma: "s \<in> sound_domain.gamma_state (ac_gamma cfg) (ac_init cfg)"
   assumes td_solve_dom:
-    "TD_plain.solve_dom
-       (make_rhs_tree (to_cfg c) (ac_tf cfg) (ac_join cfg) (ac_bot cfg) (ac_init cfg))
-       (cfg_entry (to_cfg c))"
-  assumes td_cfg_in_reach:
-    "\<And>v::pp. v \<in> reach
-       (make_rhs_tree (to_cfg c) (ac_tf cfg) (ac_join cfg) (ac_bot cfg) (ac_init cfg))
-       (TD_plain_Interp_solve
-          (make_rhs_tree (to_cfg c) (ac_tf cfg) (ac_join cfg) (ac_bot cfg) (ac_init cfg))
-          (cfg_entry (to_cfg c)))
-       (cfg_entry (to_cfg c))"
+    "\<And>v. TD_plain.solve_dom
+       (make_rhs_tree (to_cfg c) (ac_tf cfg) (ac_join cfg) (ac_bot cfg) (ac_init cfg)) v"
   assumes runs: "runs_to c s t"
   shows "t \<in> sound_domain.gamma_state (ac_gamma cfg)
                   (run_analysis cfg c (cfg_exit (to_cfg c)))"
-  using runs runs_to_def pipeline_sound_runs_to[OF sound join_eq bot_eq tf_sound s_in_gamma
-          td_solve_dom td_cfg_in_reach]
+  using runs runs_toD pipeline_sound_runs_to[OF sound join_eq bot_eq tf_sound s_in_gamma
+          td_solve_dom]
   by blast
 
 theorem sign_pipeline_invariant_sound:
   assumes tf_ok:   "domain_transfer_sound gamma_sign (ac_tf (sign_analysis_config s))"
   assumes init_ok: "s \<in> sign_domain.gamma_state (ac_init (sign_analysis_config s))"
+  assumes entry_reachable:
+    "\<And>v. \<exists>es. cfg_path (to_cfg c) (cfg_entry (to_cfg c)) es v"
   assumes td_solve_dom:
-    "TD_plain.solve_dom
+    "\<And>v. TD_plain.solve_dom
        (make_rhs_tree (to_cfg c) (ac_tf (sign_analysis_config s))
           (ac_join (sign_analysis_config s)) (ac_bot (sign_analysis_config s))
-          (ac_init (sign_analysis_config s)))
-       (cfg_entry (to_cfg c))"
-  assumes td_cfg_in_reach:
-    "\<And>v::pp. v \<in> reach
-       (make_rhs_tree (to_cfg c) (ac_tf (sign_analysis_config s))
-          (ac_join (sign_analysis_config s)) (ac_bot (sign_analysis_config s))
-          (ac_init (sign_analysis_config s)))
-       (TD_plain_Interp_solve
-          (make_rhs_tree (to_cfg c) (ac_tf (sign_analysis_config s))
-            (ac_join (sign_analysis_config s)) (ac_bot (sign_analysis_config s))
-            (ac_init (sign_analysis_config s)))
-          (cfg_entry (to_cfg c)))
-       (cfg_entry (to_cfg c))"
+          (ac_init (sign_analysis_config s))) v"
   shows   "\<forall>v. cfg_collect (to_cfg c) {s} v \<le>
                     sign_domain.gamma_state
                       (run_analysis (sign_analysis_config s) c v)"
@@ -383,8 +366,8 @@ proof -
   have inv: "\<forall>v. cfg_collect (to_cfg c) {s} v \<le>
              sound_domain.gamma_state (ac_gamma (sign_analysis_config s))
                 (run_analysis (sign_analysis_config s) c v)"
-    by (rule pipeline_invariant_sound[OF sound je be tf_ok' init_ok'
-              td_solve_dom td_cfg_in_reach])
+    by (rule pipeline_invariant_sound[OF sound je be tf_ok' init_ok' entry_reachable
+              td_solve_dom])
   show ?thesis using inv by (simp add: gs_eq)
 qed
 
